Arity-based eta-expansion proof done (assuming a suitable Aeta_expand_transform)

Launchbury/ArityEtaExpand.thy
@@ -5,11 +5,10 @@ begin
 locale ArityEtaExpand = CorrectArityAnalysisAheap +
   fixes Aeta_expand_transform :: "Arity \<Rightarrow> exp \<Rightarrow> exp"
 begin
+  lift_definition Aeta_expand :: "Arity \<Rightarrow> exp \<Rightarrow> exp"  is "\<lambda> a e. eta_expand a e".
 
-  definition Aeta_expand :: "Arity \<Rightarrow> exp \<Rightarrow> exp" 
-    where "Aeta_expand a e = eta_expand (Rep_Arity a) e"
   lemma Aeta_expand_0[simp]: "Aeta_expand 0 e = e"
-    unfolding Aeta_expand_def by (metis eta_expand.simps(1) zero_Arity.rep_eq)
+    by transfer simp
 
   lemma Aeta_expand_correct:
     assumes "ae ` upds S \<subseteq> {up \<cdot> 0}"  
@@ -23,17 +22,22 @@ begin
     from assms(2)
     have "Rep_Arity a \<le> Rep_Arity (Astack ae S)" by (metis below_Arity.rep_eq)
     finally
-    show ?thesis unfolding Aeta_expand_def by (rule eta_expansion_correct')
+    show ?thesis by transfer (rule eta_expansion_correct')
   qed
 
   lemma isLam_Aeta_expand: "isLam e \<Longrightarrow> isLam (Aeta_expand a e)"
-    unfolding Aeta_expand_def by (rule isLam_eta_expand)
+    by transfer (rule isLam_eta_expand)
+
+  lemma Aeta_expand_fresh[simp]: "a \<sharp> Aeta_expand n e = a \<sharp> e" by transfer simp
+  lemma Aeta_expand_fresh_star[simp]: "a \<sharp>* Aeta_expand n e = a \<sharp>* e" by (auto simp add: fresh_star_def)
 
   fun Aeta_expand' :: "Arity\<^sub>\<bottom> \<Rightarrow> exp \<Rightarrow> exp" 
   where "Aeta_expand' (Iup a) e = Aeta_expand a e"
    |    "Aeta_expand' Ibottom e = e"
 
   lemma [simp]: "Aeta_expand' (up\<cdot>a) e = Aeta_expand a e" unfolding up_def by (simp add: cont_Iup)
+  lemma Aeta_expand'_fresh[simp]: "a \<sharp> Aeta_expand' n e = a \<sharp> e" by (cases "(n, e)" rule: Aeta_expand'.cases) auto
+  lemma Aeta_expand'_fresh_star[simp]: "a \<sharp>* Aeta_expand' n e = a \<sharp>* e" by (auto simp add: fresh_star_def)
 
   fun Aeta_expand_transform' :: "Arity\<^sub>\<bottom> \<Rightarrow> exp \<Rightarrow> exp" 
   where "Aeta_expand_transform' (Iup a) e = Aeta_expand_transform a e"
@@ -47,17 +51,38 @@ begin
      Aeta_expand_transform a e,
      S)"
 
+  (*
   inductive consistent  where
-    [intro!]: "AE_consistent ae (\<Gamma>, e, S) \<Longrightarrow> Astack ae S \<sqsubseteq> a \<Longrightarrow> consistent (ae, a) (\<Gamma>, e, S)"
+    [intro!]: "AE_consistent ae (\<Gamma>, e, S) \<Longrightarrow> Astack ae S \<sqsubseteq> a \<Longrightarrow> Aexp e \<cdot> a \<sqsubseteq> ae \<Longrightarrow> consistent (ae, a) (\<Gamma>, e, S)"
   declare consistent.cases[elim!]
+  *)
+  
+  inductive consistent :: "(AEnv \<times> Arity) \<Rightarrow> conf \<Rightarrow> bool" where
+    consistentI[intro!]: 
+    "edom ae \<subseteq> domA \<Gamma> \<union> upds S
+    \<Longrightarrow> upds S \<subseteq> edom ae
+    \<Longrightarrow> Astack ae S \<sqsubseteq> a
+    \<Longrightarrow> AEstack ae S \<sqsubseteq> ae 
+    \<Longrightarrow> Aexp e \<cdot> a \<sqsubseteq> ae
+    \<Longrightarrow> (\<And> x e. map_of \<Gamma> x = Some e \<Longrightarrow> Aexp' e \<cdot> (ae x) \<sqsubseteq> ae)
+    \<Longrightarrow> (\<And> x e. map_of \<Gamma> x = Some e \<Longrightarrow> \<not> isLam e \<Longrightarrow> ae x = up\<cdot>0)
+    \<Longrightarrow> ae ` upds S \<subseteq> {up\<cdot>0}
+    \<Longrightarrow> consistent (ae, a) (\<Gamma>, e, S)"  
+  inductive_cases consistentE[elim!]: "consistent (ae, a) (\<Gamma>, e, S)"
+
 
   lemma [simp]:
     "Aeta_expand_transform a (App e x) = App (Aeta_expand_transform (inc\<cdot>a) e) x"
     "Aeta_expand_transform a (Lam [x]. e) = Lam [x].(Aeta_expand_transform (pred\<cdot>a) e)"
-    "Aeta_expand_transform a (e[x ::= z]) = (Aeta_expand_transform a e)[x ::= z]"
     "Aeta_expand_transform a (Var x) = Var x"
+    "Aeta_expand_transform a (Terms.Let \<Delta> e) = Terms.Let (map_ran (\<lambda>x ea. Aeta_expand' ((Aheap \<Delta>\<cdot>(Aexp e\<cdot>a)) x) (Aeta_expand_transform' ((Aheap \<Delta>\<cdot>(Aexp e\<cdot>a)) x) ea)) \<Delta>) (Aeta_expand_transform a e)"
     "isLam (Aeta_expand_transform a e) \<longleftrightarrow> isLam e"
+    "Aeta_expand_transform a (e[x ::= z]) = (Aeta_expand_transform a e)[x ::= z]"
+    "at \<sharp> Aeta_expand_transform a e \<longleftrightarrow> at \<sharp> e"
     sorry
+
+  lemma Aeta_expand_transform'_fresh[simp]: "a \<sharp> Aeta_expand_transform' n e = a \<sharp> e" by (cases "(n, e)" rule: Aeta_expand_transform'.cases) auto
+  lemma Aeta_expand_transform'_fresh_star[simp]: "a \<sharp>* Aeta_expand_transform' n e = a \<sharp>* e" by (auto simp add: fresh_star_def)
 
   sublocale AbstractConforms step consistent.
 
@@ -68,41 +93,38 @@ lemma foo:
 using assms
 proof(induction)
 case (app\<^sub>1 \<Gamma> e x S)
-  from app\<^sub>1 have "AE_consistent ae (\<Gamma>, e, Arg x # S)"  by (fastforce intro!: AE_consistentI simp add: Aexp_App join_below_iff)
-  moreover
-  have "Astack ae (Arg x # S) \<sqsubseteq> inc\<cdot>a" using app\<^sub>1 by (auto intro: monofun_cfun_arg)
-  ultimately
-  have "consistent (ae, inc\<cdot>a) (\<Gamma>, e, Arg x # S)" ..
+  from app\<^sub>1 have "consistent (ae, inc\<cdot>a) (\<Gamma>, e, Arg x # S)"  by (fastforce simp add: Aexp_App join_below_iff)
   moreover
   have "Atransform (ae, a) (\<Gamma>, App e x, S) \<Rightarrow> Atransform (ae, inc\<cdot>a) (\<Gamma>, e, Arg x # S)" by simp rule
   ultimately
-  show ?case by blast
+  show ?case by (blast del: consistentI consistentE)
 next
 case (app\<^sub>2 \<Gamma> y e x S)
-  hence "AE_consistent ae (\<Gamma>, e[y::=x], S)" 
-    by (fastforce intro!: AE_consistentI  below_trans[OF monofun_cfun_fun[OF Aexp_subst_App_Lam]] simp add: Aexp_App join_below_iff)
-  moreover
-  have "Astack ae S \<sqsubseteq> pred\<cdot>a" using app\<^sub>2 by (auto, metis monofun_cfun_arg pred_inc)
-  ultimately
-  have "consistent (ae, pred\<cdot>a) (\<Gamma>, e[y ::= x], S)" ..
+  have "Aexp (e[y ::= x])\<cdot>(pred\<cdot>a) \<sqsubseteq> ae" using app\<^sub>2
+    apply (auto simp add: Aexp_Lam join_below_iff)
+    apply (rule below_trans[OF monofun_cfun_fun[OF Aexp_subst_App_Lam]])
+    apply (auto simp add: Aexp_App join_below_iff)
+    apply (cases a rule: Arity_exhaust)
+    apply (auto simp add: Aexp_Lam join_below_iff)
+    done
+  hence "consistent (ae, pred \<cdot> a) (\<Gamma>, e[y::=x], S)"  using app\<^sub>2
+    apply  (auto intro!:  below_trans[OF monofun_cfun_fun[OF Aexp_subst_App_Lam]] simp add: Aexp_App join_below_iff monofun_cfun_arg)
+    by (metis image_eqI singletonD subsetCE)
   moreover
   have "Atransform (ae, a) (\<Gamma>, Lam [y]. e, Arg x # S) \<Rightarrow> Atransform (ae, pred \<cdot> a) (\<Gamma>, e[y::=x], S)" by simp rule
   ultimately
-  show ?case by blast
+  show ?case by (blast del: consistentI consistentE)
 next
 case (var\<^sub>1 \<Gamma> x e S)
-  from var\<^sub>1 have "Aexp (Var x)\<cdot>(Astack ae S) \<sqsubseteq> ae" by auto
+  (*
+  from var\<^sub>1 have "Aexp (Var x)\<cdot>a \<sqsubseteq> ae" by auto
   from below_trans[OF Aexp_Var fun_belowD[OF this] ]
-  have "up\<cdot>(Astack ae S) \<sqsubseteq> ae x".
-  then obtain u where "ae x = up\<cdot>u" and "Astack ae S \<sqsubseteq> u" by (cases "ae x") auto
+  have "up\<cdot>a \<sqsubseteq> ae x".
+  then obtain u where "ae x = up\<cdot>u" and "a \<sqsubseteq> u" by (cases "ae x") auto
   moreover
   hence "x \<in> edom ae" unfolding edom_def by auto
-  ultimately
-  have "AE_consistent ae (delete x \<Gamma>, e, Upd x # S)" using var\<^sub>1 by (fastforce intro!: AE_consistentI  simp add: join_below_iff)
-  moreover
-  have "Astack ae (Upd x # S) \<sqsubseteq> 0" by simp
-  ultimately
-  have "consistent (ae, 0) (delete x \<Gamma>, e, Upd x # S)" by blast
+  *)
+  have "consistent (ae, 0) (delete x \<Gamma>, e, Upd x # S)" using var\<^sub>1 by (fastforce  simp add: join_below_iff)
   moreover
   {
   from var\<^sub>1 have "ae x = up\<cdot>0" by auto
@@ -114,26 +136,26 @@ case (var\<^sub>1 \<Gamma> x e S)
     by (auto simp add: map_ran_delete intro!: step.intros)
   }
   ultimately
-  show ?case by blast
+  show ?case by (blast del: consistentI consistentE)
 next 
 case (var\<^sub>2 \<Gamma> x e S)
   from var\<^sub>2 have "ae ` upds S \<subseteq> {up \<cdot> 0}" by fastforce
 
-  from var\<^sub>2 have "Aexp (Var x)\<cdot>(Astack ae S) \<sqsubseteq> ae" by auto
+  from var\<^sub>2 have "Aexp (Var x)\<cdot>a \<sqsubseteq> ae" by auto
   from below_trans[OF Aexp_Var fun_belowD[OF this] ]
-  have "up\<cdot>(Astack ae S) \<sqsubseteq> ae x".
-  then obtain u where "ae x = up\<cdot>u" and "Astack ae S \<sqsubseteq> u" by (cases "ae x") auto
+  have "up\<cdot>a \<sqsubseteq> ae x".
+  then obtain u where "ae x = up\<cdot>u" and "a \<sqsubseteq> u" by (cases "ae x") auto
 
   from this(2)
-  have "Aexp e\<cdot>(Astack ae S) \<sqsubseteq> Aexp e\<cdot>u" by (rule monofun_cfun_arg)
+  have "Aexp e\<cdot>a \<sqsubseteq> Aexp e\<cdot>u" by (rule monofun_cfun_arg)
   also have "\<dots> \<sqsubseteq> ae" using `ae x = up \<cdot> u` var\<^sub>2 by fastforce
-  finally have "Aexp e\<cdot>(Astack ae S) \<sqsubseteq> ae" by this simp
-  hence "AE_consistent ae ((x, e) # delete x \<Gamma>, e, S)"
-    using var\<^sub>2 by(fastforce intro!: AE_consistentI  simp add: join_below_iff split:if_splits)
+  finally have "Aexp e\<cdot>a \<sqsubseteq> ae" by this simp
   moreover
-  have "Astack ae S \<sqsubseteq> u" by fact
+  have "Aexp' e\<cdot>(ae x) \<sqsubseteq> ae" using var\<^sub>2 by auto
+  hence "Aexp e\<cdot>u \<sqsubseteq> ae" using `ae x = up\<cdot>u` by simp
   ultimately
-  have "consistent (ae, u) ((x, e) # delete x \<Gamma>, e, S)" by auto
+  have "consistent (ae, u) ((x, e) # delete x \<Gamma>, e, S)"
+    using var\<^sub>2 by (auto  simp add: join_below_iff split:if_splits intro: below_trans[OF _ `a \<sqsubseteq> u`])
   moreover
   {
   from `isLam e`
@@ -150,46 +172,156 @@ case (var\<^sub>2 \<Gamma> x e S)
     using `ae x = up \<cdot> u` by (auto intro: step.intros simp add: map_ran_delete)
   also
   have "\<dots> \<Rightarrow>\<^sup>* Atransform (ae, u) ((x, e) # delete x \<Gamma>, e, S)"
-    using `ae x = up \<cdot> u` by simp (rule Aeta_expand_correct[OF `ae \` upds S \<subseteq> {up \<cdot> 0}` `Astack ae S \<sqsubseteq> u`])
+    using `ae x = up \<cdot> u`
+    apply simp
+    apply (rule Aeta_expand_correct[OF `ae \` upds S \<subseteq> {up \<cdot> 0}` below_trans[OF _ `a \<sqsubseteq> u`]])
+    using var\<^sub>2 by auto
   finally
   have "Atransform (ae, a) (\<Gamma>, Var x, S) \<Rightarrow>\<^sup>* Atransform (ae, u) ((x, e) # delete x \<Gamma>, e, S)".
   }
-  ultimately show ?case by blast
+  ultimately show ?case by (blast del: consistentI consistentE)
 next
 case (var\<^sub>3 x \<Gamma> e S)
   hence "ae x = up\<cdot>0" by auto
 
-  have "up\<cdot>(Astack ae S) \<sqsubseteq> ae x" using var\<^sub>3 by (auto simp add: join_below_iff)
-  then obtain u where "ae x = up \<cdot> u" and "Astack ae S \<sqsubseteq> u" by (cases "ae x") auto
-
-  have "Aexp e\<cdot>(Astack ae S) \<sqsubseteq> Aexp e\<cdot>0" by (rule monofun_cfun_arg) simp
-  also have "\<dots> \<sqsubseteq> ae" using `ae x = up \<cdot> 0` var\<^sub>3 by auto
-  finally have "Aexp e\<cdot>(Astack ae S) \<sqsubseteq> ae" by this simp
-  hence "AE_consistent ae ((x, e) # \<Gamma>, e, S)" using var\<^sub>3 `ae x = up \<cdot> 0`
-    by (fastforce intro!: AE_consistentI  simp add: join_below_iff split:if_splits)+
-  moreover
   have "Astack ae (Upd x # S) \<sqsubseteq> a" using var\<^sub>3 by auto
   with `ae x = up \<cdot> 0`
   have "a = 0" by auto
-  
-  have "Astack ae S \<sqsubseteq> 0" by simp
-  ultimately
-  have "consistent (ae, 0) ((x, e) # \<Gamma>, e, S)" by auto
+
+  have "consistent (ae, 0) ((x, e) # \<Gamma>, e, S)" using var\<^sub>3 
+    by (fastforce  simp add: join_below_iff split:if_splits)
   moreover
   have "Atransform (ae, a) (\<Gamma>, e, Upd x # S) \<Rightarrow> Atransform (ae, 0) ((x, e) # \<Gamma>, e, S)"
     using `ae x = up\<cdot>0` `a = 0` var\<^sub>3 by (fastforce intro!: step.intros)
-  ultimately show ?case by blast
+  ultimately show ?case by (blast del: consistentI consistentE)
 next
   case (let\<^sub>1 \<Delta> \<Gamma> S e)
 
-  show ?case sorry
+  let ?ae = "Aheap \<Delta> \<cdot> (Aexp e\<cdot>a)"
+  let ?new = "(domA (\<Delta> @ \<Gamma>) \<union> upds S - (domA \<Gamma> \<union> upds S))"
+  have new: "?new = domA \<Delta>"
+    using fresh_distinct[OF let\<^sub>1(1)] fresh_distinct_fv[OF let\<^sub>1(2)]
+    by (auto dest: set_mp[OF ups_fv_subset])
+
+  have "domA \<Delta> \<inter> upds S = {}" using fresh_distinct_fv[OF let\<^sub>1(2)] by (auto dest: set_mp[OF ups_fv_subset])
+  hence *: "\<And> x. x \<in> upds S \<Longrightarrow> x \<notin> edom (Aheap \<Delta>\<cdot>(Aexp e\<cdot>a))"
+    using edom_Aheap[where \<Gamma> = \<Delta> and ae = "Aexp e\<cdot>a"] by auto
+  hence stack: "AEstack (Aheap \<Delta>\<cdot>(Aexp e\<cdot>a) \<squnion> ae) S = AEstack ae S"
+               "Astack (Aheap \<Delta>\<cdot>(Aexp e\<cdot>a) \<squnion> ae) S = Astack ae S"
+    by (auto simp add: edomIff cong: AEstack_cong Astack_cong)
+
+
+  have "edom ae \<subseteq> - domA \<Delta>" using let\<^sub>1(3)
+    using fresh_distinct[OF let\<^sub>1(1)] fresh_distinct_fv[OF let\<^sub>1(2)]
+    by (fastforce dest: set_mp[OF ups_fv_subset])
+  hence "(?ae \<squnion> ae) f|` (- domA \<Delta>) = ae"
+    by (auto simp add: env_restr_join  env_restr_useless disjoint_eq_subset_Compl edom_Aheap)
+  moreover
+  {
+  have "edom (?ae \<squnion> ae) \<subseteq> domA (\<Delta> @ \<Gamma>) \<union> upds S"
+    using let\<^sub>1(3) by (auto dest: set_mp[OF edom_Aheap])
+  moreover
+  have "upds S \<subseteq> edom (?ae \<squnion> ae)"
+    using let\<^sub>1(3) by auto
+  moreover
+  have "AEstack ae S \<sqsubseteq> ae" using let\<^sub>1(3) by auto
+  hence "AEstack ae S \<sqsubseteq> ?ae \<squnion> ae" by (metis join_above1 below_refl box_below join_comm)
+  moreover
+  { fix x e'
+    assume "map_of \<Delta> x = Some e'"
+    hence "x \<notin> edom ae" using `edom ae \<subseteq> - domA \<Delta>` by (metis Compl_iff contra_subsetD domI dom_map_of_conv_domA)
+    hence "Aexp' e'\<cdot>((?ae \<squnion> ae) x) = Aexp' e'\<cdot>(?ae x)" by (auto simp add: edomIff)
+    also
+    have "Aexp' e'\<cdot>(?ae x) \<sqsubseteq> (Aexp' e'\<cdot>(?ae x) f|` domA \<Delta>) \<squnion> (Aexp' e'\<cdot>(?ae x) f|` (- domA \<Delta>))"
+      by (rule eq_imp_below[OF join_env_restr_UNIV[symmetric]]) auto
+    also
+    from `map_of \<Delta> x = Some e'`
+    have "Aexp' e'\<cdot>(?ae x) f|` domA \<Delta> \<sqsubseteq> ?ae" by (rule Aheap_heap)
+    also
+    from `map_of \<Delta> x = Some e'`
+    have "Aexp' e'\<cdot>(?ae x) f|` (- domA \<Delta>) \<sqsubseteq> Aexp (Terms.Let \<Delta> e)\<cdot>a" by (rule Aheap_heap2)
+    also
+    have "Aexp (Terms.Let \<Delta> e)\<cdot>a \<sqsubseteq> ae" using let\<^sub>1(3) by auto
+    finally
+    have "Aexp' e'\<cdot>((?ae \<squnion> ae) x) \<sqsubseteq> ?ae \<squnion> ae" by this auto
+  }
+  moreover
+  { fix x e'
+    assume "map_of \<Gamma> x = Some e'"
+    hence "x \<in> domA \<Gamma>" by (metis domI dom_map_of_conv_domA)
+    hence "x \<notin> edom ?ae" using fresh_distinct[OF let\<^sub>1(1)]  by (auto dest: set_mp[OF edom_Aheap])
+    with let\<^sub>1 `map_of \<Gamma> x = Some e'`
+    have "Aexp' e'\<cdot>((?ae \<squnion> ae) x) \<sqsubseteq> ae" by (auto simp add: edomIff)
+    hence "Aexp' e'\<cdot>((?ae \<squnion> ae) x) \<sqsubseteq> ?ae \<squnion> ae" by (metis (erased, hide_lams) "HOLCF-Join-Classes.join_above2" below_trans)
+  }
+  moreover
+  { fix x e'
+    assume "\<not> isLam e'"
+    assume "map_of \<Gamma> x = Some e'"
+    hence "x \<in> domA \<Gamma>" by (metis domI dom_map_of_conv_domA)
+    hence "x \<notin> edom ?ae" using fresh_distinct[OF let\<^sub>1(1)]  by (auto dest: set_mp[OF edom_Aheap])
+    with let\<^sub>1 `map_of \<Gamma> x = Some e'` `\<not> isLam e'`
+    have "(?ae \<squnion> ae) x = up \<cdot>0" by (auto simp add: edomIff)
+  }
+  moreover
+  { fix x e'
+    assume "map_of \<Delta> x = Some e'" and "\<not> isLam e'"
+    hence "?ae x = up \<cdot> 0" using Aheap_heap3 by auto
+    hence "(?ae \<squnion> ae) x = up \<cdot> 0" by simp
+  }
+  moreover
+  have "(?ae \<squnion> ae) ` upds S \<subseteq> {up \<cdot> 0}" using let\<^sub>1 * by fastforce
+  moreover
+  have "Astack (?ae \<squnion> ae) S \<sqsubseteq> a" unfolding stack using let\<^sub>1 by auto
+  moreover
+  {
+  have "Aexp e\<cdot>a \<sqsubseteq> (Aexp e\<cdot>a f|` domA \<Delta>) \<squnion> (Aexp e\<cdot>a f|` (- domA \<Delta>))"
+    by (rule eq_imp_below[OF join_env_restr_UNIV[symmetric]]) auto
+  also have "Aexp e\<cdot>a f|` (- domA \<Delta>) \<sqsubseteq> Aexp (Terms.Let \<Delta> e)\<cdot>a" by (rule Aexp_Let_above)
+  also have "\<dots> \<sqsubseteq> ae" using let\<^sub>1(3) by auto
+  also have "Aexp e\<cdot>a f|` domA \<Delta> \<sqsubseteq> ?ae" by (rule Aheap_above_arg)
+  finally have "Aexp e\<cdot>a \<sqsubseteq> ?ae \<squnion> ae" by this auto
+  }
+  ultimately
+  have "consistent (?ae \<squnion> ae, a) (\<Delta> @ \<Gamma>, e, S) "
+    by (auto  simp add: stack)
+  }
+  moreover
+  {
+    have "\<And> x. x \<in> set \<Gamma> \<Longrightarrow> fst x \<notin> edom (Aheap \<Delta>\<cdot>(Aexp e\<cdot>a))"
+      using fresh_distinct[OF let\<^sub>1(1)]
+      by (auto dest!: set_mp[OF edom_Aheap] domA_from_set)
+    hence "map_ran (\<lambda>x ea. Aeta_expand' ((Aheap \<Delta>\<cdot>(Aexp e\<cdot>a)) x \<squnion> ae x) (Aeta_expand_transform' ((Aheap \<Delta>\<cdot>(Aexp e\<cdot>a)) x \<squnion> ae x) ea)) \<Gamma>
+       = map_ran (\<lambda>x ea. Aeta_expand' (ae x) (Aeta_expand_transform' (ae x) ea)) \<Gamma>"
+      by (auto intro: map_ran_cong[OF _ refl] simp add: edomIff)
+    moreover
+    from let\<^sub>1 have *: "edom ae \<subseteq> domA \<Gamma> \<union> upds S" by auto
+    have "\<And> x. x \<in> set \<Delta> \<Longrightarrow> fst x \<notin> edom ae"
+       using fresh_distinct[OF let\<^sub>1(1)] fresh_distinct_fv[OF let\<^sub>1(2)] 
+       by (auto dest!: set_mp[OF *] set_mp[OF ups_fv_subset] domA_from_set)
+    hence "map_ran (\<lambda>x ea. Aeta_expand' ((Aheap \<Delta>\<cdot>(Aexp e\<cdot>a)) x \<squnion> ae x) (Aeta_expand_transform' ((Aheap \<Delta>\<cdot>(Aexp e\<cdot>a)) x \<squnion> ae x) ea)) \<Delta>
+       = map_ran (\<lambda>x ea. Aeta_expand' ((Aheap \<Delta>\<cdot>(Aexp e\<cdot>a)) x) (Aeta_expand_transform' ((Aheap \<Delta>\<cdot>(Aexp e\<cdot>a)) x) ea)) \<Delta>"
+      by (auto intro: map_ran_cong[OF _ refl]  simp add: edomIff)
+    ultimately
+    have "Atransform (ae, a) (\<Gamma>, Terms.Let \<Delta> e, S) \<Rightarrow> Atransform (?ae \<squnion> ae, a) (\<Delta> @ \<Gamma>, e, S)"
+      apply (simp add: map_ran_append)
+      apply rule
+      using let\<^sub>1(1,2)
+      apply auto
+      apply (induction \<Gamma>)
+      apply simp
+      apply (auto simp add: fresh_star_Pair fresh_star_Cons)
+      done
+  }
+  ultimately
+  show ?case  by (blast del: consistentI consistentE)
 qed
 
 
   sublocale AbstractTransform step consistent Atransform
     apply default
     using foo
-    apply blast
+    apply (auto del: consistentI consistentE)
     done
 
 end
