Launchbury/AList-Utils.thy
@@ -98,7 +98,7 @@ lemma ran_map_cong[fundef_cong]:
       \<Longrightarrow> map_ran f1 m1 = map_ran f2 m2"    
   by (induction rule: list_all2_induct) auto
 *)
-lemma ran_map_cong[fundef_cong]:
+lemma map_ran_cong[fundef_cong]:
   "\<lbrakk> \<And> x . x \<in> set m1 \<Longrightarrow> f1 (fst x) (snd x) = f2 (fst x) (snd x) ; m1 = m2 \<rbrakk>
       \<Longrightarrow> map_ran f1 m1 = map_ran f2 m2"    
   by (induction m1 arbitrary: m2) auto
@@ -108,6 +108,10 @@ lemma domA_map_ran[simp]: "domA (map_ran f m) = domA m"
 
 lemma map_ran_delete:
   "map_ran f (delete x \<Gamma>) = delete x (map_ran f \<Gamma>)"
+  by (induction \<Gamma>)  auto
+
+lemma map_ran_append:
+  "map_ran f (\<Gamma>@\<Delta>) = map_ran f \<Gamma> @ map_ran f \<Delta>"
   by (induction \<Gamma>)  auto
 
 end
