Launchbury/ArityCorrect.thy
@@ -26,6 +26,7 @@ end
 locale CorrectArityAnalysis = EdomArityAnalysis +
   assumes Aexp_Var: "up \<cdot> n \<sqsubseteq> (Aexp (Var x) \<cdot> n) x"
   assumes Aexp_subst_App_Lam: "Aexp (e[y::=x]) \<sqsubseteq> Aexp (App (Lam [y]. e) x)"
+  assumes Aexp_Lam: "Aexp (Lam [y]. e) \<cdot> n = env_delete y (Aexp e \<cdot>(pred\<cdot>n))
   assumes Aexp_App: "Aexp (App e x) \<cdot> n = Aexp e \<cdot>(inc\<cdot>n) \<squnion> AE_singleton x \<cdot> (up\<cdot>0)"
 
 locale CorrectArityAnalysisAfix = CorrectArityAnalysis + 
